Metrology/ProbLang.lean
@@ -1,3 +1,4 @@
 import Metrology.ProbLang.Syntax
 import Metrology.ProbLang.Opsem
 import Metrology.ProbLang.PrimStep
+import Metrology.ProbLang.PureStep
